$RD_{\circ} (1) = \{(x, ?), (y, ?), (z, ?), (t, ?), (i, ?)\}$

$RD_{\bullet} (1) = RD_{\circ} (1) \setminus \{(x, l) | l \in Lab \} \cup \{(x, 1)\}$

$RD_{\circ} (2) = RD_{\bullet} (1)$

$RD_{\bullet} (2) = RD_{\circ} (2) \setminus \{(y, l) | l \in Lab \} \cup \{(y, 2)\}$

$RD_{\circ} (3) = RD_{\bullet} (2)$

$RD_{\bullet} (3) = RD_{\circ} (3) \setminus \{(i, l) | l \in Lab \} \cup \{(i, 3)\}$

$RD_{\circ} (4) = RD_{\bullet} (3) \cup\ RD_{\bullet} (8)$

$RD_{\bullet} (4) = RD_{\circ} (4)$

$RD_{\circ} (5) = RD_{\bullet} (4)$

$RD_{\bullet} (5) = RD_{\circ} (5) \setminus \{(t, l) | l \in Lab \} \cup \{(t, 5)\}$

$RD_{\circ} (6) = RD_{\bullet} (5)$

$RD_{\bullet} (6) = RD_{\circ} (6) \setminus \{(x, l) | l \in Lab \} \cup \{(x, 6)\}$

$RD_{\circ} (7) = RD_{\bullet} (6)$

$RD_{\bullet} (7) = RD_{\circ} (7) \setminus \{(y, l) | l \in Lab \} \cup \{(y, 7)\}$

$RD_{\circ} (8) = RD_{\bullet} (7)$

$RD_{\bullet} (8) = RD_{\circ} (8) \setminus \{(i, l) | l \in Lab \} \cup \{(i, 8)\}$

$RD_{\circ} (9) = RD_{\bullet} (4)$

$RD_{\bullet} (9) = RD_{\circ} (9) \setminus \{(y, l) | l \in Lab \} \cup \{(y, 9)\}$
